src/semantics.lean
@@ -2,25 +2,29 @@
 
 import process
 
+universe u
+
+open objects
+
 /- A local configuration is an object and its process. -/
 @[derive decidable_eq]
-structure local_config (α β : Type) [interpret α β]
+structure local_config {α β : Type} [interpret α β]
   (C : class_name α) := (σ : Σ(C)) (m : process C)
+
 /- A global configuration is a finite set of object configurations and a global history. -/
 @[derive decidable_eq]
 structure global_config (α β : Type) [interpret α β] :=
-  --(Γ: finset (local_config α β))
+  (Γ (C : class_name α): finset (local_config C))
   (θ: global_history α β)
 
 /- A step is taken on a local configuration. -/
 def local_config.step {α β : Type} [interpret α β]
     (p : program α) (C : class_name α)
     (θ : global_history α β) :
-    local_config α β C → set (local_config α β C)
+    local_config C → set (local_config C)
 /- If the process is inactive, we obtain a pending method call. If no method call is pending, no step is taken. Otherwise, the next local configuration is an active process with the arguments of the selected method, a default store, and the body of the method as statement; additionally, a selection event is generated. -/
 | ⟨σ, process.nil _⟩ := let e := θ.sched σ.id in option.elim e
     (λ_, ∅) (λd h, {⟨σ, process.schedule p σ d h⟩})
-    -- TODO (event.selection d)
 /- Otherwise, there is an active process. We look at the list of statements. If the list is empty, the process becomes inactive. -/
 | ⟨σ, process.active ⟨e,τ,ℓ,[]⟩⟩ := {⟨σ, process.nil _⟩}
 /- Otherwise, there is a current statement. If the current statement is an if statement, for which we evaluate the boolean pure expression. If it is true, we replace the current statement by those of the then-branch. Otherwise, we replace the current statement by those of the else-branch. -/
@@ -46,22 +50,96 @@ def local_config.step {α β : Type} [interpret α β]
     {⟨σ, process.active ⟨e,τ,ℓ.update l (eval σ π p).the,t⟩⟩}
 /- Otherwise, we have an async statement. We evaluate the argument list to a value list; the object pure expression is evaluated to an object value. If that value is null, no step is taken. Otherwise, we generate a method selection event with our object as caller and the appropriate call site, and discard the current statement. -/
 | ⟨σ, process.active π@⟨e,τ,ℓ,(stmt.async c m G o τ' :: t)⟩⟩ :=
-    (π.lookup σ o).elim_object
-      (λo h, {⟨σ, process.active ⟨e,τ,ℓ,t⟩⟩})
-      -- TODO (event.call σ.id ⟨o,m,eval σ π τ'⟩)
-      (λ_, ∅)
+    match (π.lookup σ o) with
+    | value.null _ := ∅
+    | value.object _ := {⟨σ, process.active ⟨e,τ,ℓ,t⟩⟩}
+    end
 /- Otherwise, we have an alloc statement. We evaluate the argument list to a value list. A fresh object identity is obtained from the global history, and stored in the variable. A call event to the constructor of the freshly obtained object is generated with an approriate call site, and the current statement is discarded. -/
 | ⟨σ, process.active
       π@⟨e,τ,ℓ,(stmt.alloc c (svar.fvar f) τ' :: t)⟩⟩ :=
-    {r : local_config α β C |
-    ∃o : {o // c = objects.class_of α o}, θ.fresh o ∧
-    let new := value.object o in
-      r = ⟨σ.updatev f new, process.active ⟨e,τ,ℓ,t⟩⟩}
+    λr : local_config C, ∃o : {o : β // c = class_of α o},
+      θ.fresh o ∧ let new := value.object o in
+        r = ⟨σ.updatev f new, process.active ⟨e,τ,ℓ,t⟩⟩
     -- TODO (event.call σ.id ⟨o,ctor c,eval σ π τ'⟩
 | ⟨σ, process.active 
       π@⟨e,τ,ℓ,(stmt.alloc c (svar.lvar ⟨l⟩) τ' :: t)⟩⟩ :=
-    {r : local_config α β C |
-    ∃o : {o // c = objects.class_of α o}, θ.fresh o ∧
-    let new := value.object o in
-      r = ⟨σ, process.active ⟨e,τ,ℓ.update l new,t⟩⟩}
+    λr : local_config C, ∃o : {o // c = class_of α o},
+      θ.fresh o ∧ let new := value.object o in
+        r = ⟨σ, process.active ⟨e,τ,ℓ.update l new,t⟩⟩
     -- TODO (event.call σ.id ⟨o,ctor c,eval σ π τ'⟩)
+
+/- Fact: after a local configuration takes a step that results in the allocation of an object, that object's identity is stored in the resulting local configuration. We have that object identities are encodable, and this crucially allows us to make use of constructive choice. -/
+def local_config.last_falloc {α β : Type} [interpret α β]
+    {p : program α} {C : class_name α}
+    {θ : global_history α β}
+    (r : local_config C)
+    {σ : Σ(C)} {e : tenv C} {τ : vallist (tenv.args e)}
+    {ℓ : vallist (e.locals)}
+    {c : class_name α} {f : fvar e (type.ref c)}
+    {τ' : pexp e (param_types (ctor c))}
+    {t : list (statement e)}
+    (R : local_config.step p C θ ⟨σ, process.active
+      ⟨e,τ,ℓ,(stmt.alloc c (svar.fvar f) τ' :: t)⟩⟩ r) :
+    {o : β // c = class_of α o} :=
+begin
+  simp [local_config.step] at R, 
+  exact (let o := (encodable.choose R) in ⟨o, begin
+    have : θ.fresh o ∧ ∃(H : c = class_of α o), _,
+      apply encodable.choose_spec R,
+    cases this, cases this_right, assumption
+  end⟩)
+end
+def local_config.last_lalloc {α β : Type} [interpret α β]
+    {p : program α} {C : class_name α}
+    {θ : global_history α β}
+    (r : local_config C)
+    {σ : Σ(C)} {e : tenv C} {τ : vallist (tenv.args e)}
+    {ℓ : vallist (e.locals)}
+    {c : class_name α} {l : list_at (type.ref c) (e.locals)}
+    {τ' : pexp e (param_types (ctor c))}
+    {t : list (statement e)}
+    (R : local_config.step p C θ ⟨σ, process.active
+      ⟨e,τ,ℓ,(stmt.alloc c (svar.lvar ⟨l⟩) τ' :: t)⟩⟩ r) :
+    {o : β // c = class_of α o} :=
+begin
+  simp [local_config.step] at R, 
+  exact (let o := (encodable.choose R) in ⟨o, begin
+    have : θ.fresh o ∧ ∃(H : c = class_of α o), _,
+      apply encodable.choose_spec R,
+    cases this, cases this_right, assumption
+  end⟩)
+end
+
+def local_config.effect {α β : Type} [interpret α β]
+    {p : program α} {C : class_name α}
+    {θ : global_history α β}
+    {l : local_config C} {r : local_config C}
+    {R : local_config.step p C θ l r} : option (event α β) :=
+match l, rfl : (∀ b, l = b → _) with
+| ⟨σ, process.nil _⟩, _ := (θ.sched σ.id).map event.selection
+| ⟨σ, process.active
+      π@⟨e,τ,ℓ,(stmt.async c m G o τ' :: t)⟩⟩, _ :=
+    match (π.lookup σ o) with
+    | value.null _ := none
+    | value.object o := (event.call σ.id ⟨o,m,eval σ π τ'⟩)
+    end
+| ⟨σ, process.active
+      π@⟨e,τ,ℓ,(stmt.alloc c (svar.fvar f) τ' :: t)⟩⟩, H :=
+    match r with
+    | ⟨σ', process.active π'⟩ := let o :=
+          local_config.last_falloc r
+            (cast begin rewrite H end R) in
+        (event.call σ.id ⟨o,ctor c,eval σ π τ'⟩)
+    | _ := none
+    end
+| ⟨σ, process.active
+      π@⟨e,τ,ℓ,(stmt.alloc c (svar.lvar ⟨l⟩) τ' :: t)⟩⟩, H :=
+    match r with
+    | ⟨σ', process.active π'⟩ := let o :=
+          local_config.last_lalloc r
+            (cast begin rewrite H end R) in
+        (event.call σ.id ⟨o,ctor c,eval σ π τ'⟩)
+    | _ := none
+    end
+| _, _ := none
+end
